

**Solution**

To solve this integral, we will use the **_Partial Fraction Decomposition_** method. 

First, we need to factor the denominator:

$$\frac{x^3 + 6x^2 + 11x + 7}{(x^2 + 3x + 2)(x+2)} = \frac{A}{x^2 + 3x + 2} + \frac{B}{x+2}$$

To find the values of A and B, we need to multiply both sides of the equation with the product of denominators $(x^2 + 3x + 2)(x+2)$ and equate coefficients of each power of $x$:

$$x^3 + 6x^2 + 11x + 7 = A(x+2) + B(x^2 + 3x + 2)$$

Equating coefficients of $x^3$: 

$$1 = A \implies A = 1$$

Equating coefficients of $x^2$:

$$6 = 3B \implies B = 2$$

Therefore, 

$$\frac{x^3 + 6x^2 + 11x + 7}{(x^2 + 3x + 2)(x+2)} = \frac{1}{x^2 + 3x + 2} + \frac{2}{x+2}$$

Now, we will integrate both the fractions separately:

$$\int \frac{1}{x^2 + 3x + 2} dx = \int \frac{1}{(x+2)(x+1)} dx$$

Using the **_Substitution Method_**:

Let $u = x+2 \implies du = dx$

$$\int \frac{1}{(x+2)(x+1)} dx = \int \frac{1}{u(u-1)} du$$

$$\int \frac{1}{u(u-1)} du = \int \frac{1}{u} - \frac{1}{u-1} du$$

$$= \ln|u| - \ln|u-1| + c$$

Substituting back the value of $u$, 

$$\int \frac{1}{x^2 + 3x + 2} dx = \ln|x+2| - \ln|x+1| + c$$

Similarly,

$$\int \frac{2}{x+2} dx = 2\ln|x+2| + c$$

Therefore,

$$\int \frac{x^3 + 6x^2 + 11x + 7}{(x^2 + 3x + 2)(x+2)} dx = \ln|x+2| - \ln|x+1| + 2\ln|x+2| + c$$

$$= \ln\left(\frac{|x+2|}{|x+1|}\right) + 2\ln|x+2| + c$$