

**Solution:**

Step 1: Make the equation canonical

We will rewrite the given equation in the form of $Ax^2 + Bxy + Cy^2 + Dx + Ey + F = 0$, by completing the square.

$$9x^2 - 16y^2 -90x + 32y - 367 = 0$$

$$9x^2 -90x + \frac{81}{4} + 16y^2 - 32y + \frac{256}{4} -367 = 0$$

$$\bigg(3x - \frac{45}{2}\bigg)^2 + \bigg(4y - \frac{16}{2}\bigg)^2 + \bigg(\frac{81}{4} - \frac{256}{4} -367\bigg) = 0$$

$$\bigg(3x - \frac{45}{2}\bigg)^2 + \bigg(4y - \frac{16}{2}\bigg)^2 - \frac{512}{4} = 0$$

$$A = 9, B = 0, C = 16, D = -90, E = -32, F = -\frac{512}{4}$$

$$9x^2 + 0xy + 16y^2 -90x -32y - \frac{512}{4} = 0$$

Step 2: Find the Center and Radius

The center of the ellipse is given by:

$$h = -\frac{D}{2A} = -\frac{(-90)}{2(9)} = 5$$

$$k = -\frac{E}{2C} = -\frac{(-32)}{2(16)} = 1$$

The radius of the ellipse is given by:

$$a = \sqrt{\frac{-F + h^2 + k^2}{A}} = \sqrt{\frac{-\frac{512}{4} + 5^2 + 1^2}{9}} = \sqrt{\frac{43}{9}} \approx 2.657$$

$$b = \sqrt{\frac{-F - h^2 - k^2}{C}} = \sqrt{\frac{-\frac{512}{4} - 5^2 - 1^2}{16}} = \sqrt{\frac{-35}{4}} \approx 2.647$$

Step 3: Find the Foci

The foci are given by:

$$F_1 = (h + a, k) = (5 + 2.657, 1) \approx (7.657, 1)$$

$$F_2 = (h - a, k) = (5 - 2.657, 1) \approx (2.343, 1)$$

Step 4: Find the Equation of the Ellipse

The equation of the ellipse is given by:

$$\bigg(\frac{x - h}{a}\bigg)^2 + \bigg(\frac{y - k}{b}\bigg)^2 = 1$$

$$\bigg(\frac{x - 5}{2.657}\bigg)^2 + \bigg(\frac{y - 1}{2.647}\bigg)^2 = 1$$

**Решение:**

Шаг 1: Делаем уравнение каноничным

Мы перепишем данное уравнение в виде $Ax^2 + Bxy + Cy^2 + Dx + Ey + F = 0$, закончив квадрат.

$$9x^2 - 16y^2 -90x + 32y - 367 = 0$$

$$9x^2 -90x + \frac{81}{4} + 16y^2 - 32y + \frac{256}{4} -367 = 0$$

$$\bigg(3x - \frac{45}{2}\bigg)^2 + \bigg(4y - \frac{16}{2}\bigg)^2 + \bigg(\frac{81}{4} - \frac{256}{4} -367\bigg) = 0$$

$$\bigg(3x - \frac{45}{2}\bigg)^2 + \bigg(4y - \frac{16}{2}\bigg)^2 - \frac{512}{4} = 0$$

$$A = 9, B = 0, C = 16, D = -90, E = -32, F = -\frac{512}{4}$$

$$9x^2 + 0xy + 16y^2 -90x -32y - \frac{512}{4} = 0$$

Шаг 2: Найдем центр и радиус

Центр эллипса дается в виде:

$$h = -\frac{D}{2A} = -\frac{(-90)}{2(9)} = 5$$

$$k = -\frac{E}{2C} = -\frac{(-32)}{2(16)} = 1$$

Радиус эллипса дается в виде:

$$a = \sqrt{\frac{-F + h^2 + k^2}{A}} = \sqrt{\frac{-\frac{512}{4} + 5^2 + 1^2}{9}} = \sqrt{\frac{43}{9}} \approx 2.657$$

$$b = \sqrt{\frac{-F - h^2 - k^2}{C}} = \sqrt{\frac{-\frac{512}{4} - 5^2 - 1^2}{16}} = \sqrt{\frac{-35}{4}} \approx 2.647$$

Шаг 3: Найдем фокусы

Фокусы даются в виде:

$$F_1 = (h + a, k) = (5 + 2.657, 1) \approx (7.657, 1)$$

$$F_2 = (h - a, k) = (5 - 2.657, 1) \approx (2.343, 1)$$

Шаг 4: Найдем уравнение эллипса

Уравнение эллипса дается в виде:

$$\bigg(\frac{x - h}{a}\bigg)^2 + \bigg(\frac{y - k}{b}\bigg)^2 = 1$$

$$\bigg(\frac{x - 5}{2.657}\bigg)^2 + \bigg(\frac{y - 1}{2.647}\bigg)^2 = 1$$