

**Solution**

The given equation is 

$$y'' - y = 6\sin2x$$

This is a second-order linear differential equation with constant coefficients and can be solved using the method of undetermined coefficients.

Let us assume the solution of the form 

$$y = A\sin2x + B\cos2x$$

Substituting this in the given equation, we get

$$A\sin2x + B\cos2x - (A\sin2x + B\cos2x) = 6\sin2x$$

This gives us

$$A\sin2x + B\cos2x - A\sin2x - B\cos2x = 6\sin2x$$

Simplifying further, we get

$$A\sin2x - A\sin2x + B\cos2x - B\cos2x = 6\sin2x$$

This yields

$$A(\sin2x - \sin2x) + B(\cos2x - \cos2x) = 6\sin2x$$

$$\implies A\cdot0 + B\cdot0 = 6\sin2x$$

Since $A$ and $B$ cannot be equal to $0$, we have

$$0 = 6\sin2x$$

This implies that

$$\sin2x = 0$$

$$\implies 2x = n\pi$$, where $n$ is any integer

Therefore, the solution of the given equation is

$$y = A\sin2x + B\cos2x$$

$$= A\sin(n\pi) + B\cos(n\pi)$$

$$= A\cdot0 + B\cdot(-1)^n$$