

### Solution: 

We can solve this integral by using partial fraction decomposition.

Let us start by writing the integral as: 

$$\int \frac{2x - 1}{x^3 - 1} dx$$

We can factor the denominator as: 

$$x^3 - 1 = (x - 1)(x^2 + x + 1)$$

Now, let us decompose the fraction as follows: 

$$ \frac{2x - 1}{x^3 - 1} = \frac{A}{x - 1} + \frac{Bx + C}{x^2 + x + 1}$$

We can multiply both sides by $x^3 - 1$ to obtain: 

$$2x - 1 = A(x^2 + x + 1) + (Bx + C)(x - 1)$$

After expanding, we get: 

$$2x - 1 = Ax^2 + (A + B)x + A + C$$

To find the values of $A$, $B$, and $C$, we can compare the coefficients of each side.

From the coefficient of $x^2$, we get: 

$$A = 2$$

From the coefficient of $x$, we get: 

$$A + B = 0 \Rightarrow B = -2$$

From the constant term, we get: 

$$A + C = -1 \Rightarrow C = -3$$

Now, we can substitute the values of $A$, $B$, and $C$ in our original expression to get: 

$$ \frac{2x - 1}{x^3 - 1} = \frac{2}{x - 1} - \frac{2x - 3}{x^2 + x + 1}$$

Integrating both sides, we get: 

$$\int \frac{2x - 1}{x^3 - 1} dx = \int \frac{2}{x - 1} dx - \int \frac{2x - 3}{x^2 + x + 1} dx$$

The first integral can be solved easily as follows: 

$$\int \frac{2}{x - 1} dx = 2 \ln |x - 1| + C$$

The second integral can be solved using trigonometric substitution as follows: 

Let $x = \tan \theta$. Then, $dx = \sec^2 \theta d\theta$. 

Substituting these values in the integral, we get: 

$$\int \frac{2x - 3}{x^2 + x + 1} dx = \int \frac{2\tan \theta - 3}{\tan^2 \theta + \tan \theta + 1} \sec^2 \theta d\theta$$

Simplifying, we get: 

$$\int \frac{2x - 3}{x^2 + x + 1} dx = \int \frac{2\sec^2 \theta - 3\sec^2 \theta}{\sec^2 \theta} d\theta = \int (2 - 3\sec^2 \theta) d\theta$$

Integrating, we get: 

$$\int (2 - 3\sec^2 \theta) d\theta = 2\theta - 3\tan \theta + C$$

Substituting $x = \tan \theta$, we get: 

$$\int \frac{2x - 3}{x^2 + x + 1} dx = 2\tan^{-1} x - 3x + C$$

Now, combining both the integrals, we get: 

$$\int \frac{2x - 1}{x^3 - 1} dx = 2 \ln |x - 1| + 2\tan^{-1} x - 3x + C$$