

**Solution**

We will solve this integral using **Substitution Method**.

Let $$u = \ln(x) \Rightarrow du = \frac{1}{x} dx$$

Substituting this in the integral, we get

$$\int \frac{dx}{x \sqrt{3 + (\ln(x))^2}} = \int \frac{du}{\sqrt{3 + u^2}}$$

Now, using the **Trigonometric Substitution**, let $$u = \tan(\theta) \Rightarrow du = \sec^2(\theta) d\theta$$

Substituting this in the integral, we get

$$\begin{align}
\int \frac{dx}{x \sqrt{3 + (\ln(x))^2}} &= \int \frac{du}{\sqrt{3 + u^2}} \\
&= \int \frac{\sec^2(\theta) d\theta}{\sqrt{3 + \tan^2(\theta)}} \\
&= \int \frac{\sec^2(\theta) d\theta}{\sqrt{3 + \sec^2(\theta)}} \\
&= \int \frac{\sec^2(\theta) d\theta}{\sqrt{3(1 + \sec^2(\theta))}} \\
&= \int \frac{\sec^2(\theta) d\theta}{\sec(\theta)\sqrt{3 + \sec^2(\theta)}} \\
&= \int \frac{d\theta}{\sqrt{3 + \sec^2(\theta)}}
\end{align}$$

Now, let $$\sec^2(\theta) = t \Rightarrow d\theta = \frac{dt}{2 \sqrt{t^2 - 1}}$$

Substituting this in the integral, we get

$$\begin{align}
\int \frac{dx}{x \sqrt{3 + (\ln(x))^2}} &= \int \frac{d\theta}{\sqrt{3 + \sec^2(\theta)}} \\
&= \int \frac{dt}{2 \sqrt{t^2 - 1}\sqrt{3 + t}}
\end{align}$$

Now, using the **Integration by Parts**, let $$u = \frac{1}{\sqrt{t^2 - 1}} \Rightarrow dv = \frac{dt}{\sqrt{3 + t}}$$

and

$$\begin{align}
du &= \frac{-1}{(t^2 - 1)^{\frac{3}{2}}} dt \\
v &= 2 \sqrt{3 + t}
\end{align}$$

Substituting this in the integral, we get

$$\begin{align}
\int \frac{dx}{x \sqrt{3 + (\ln(x))^2}} &= \int \frac{dt}{2 \sqrt{t^2 - 1}\sqrt{3 + t}} \\
&= \frac{1}{2} \left[ uv - \int v du \right] \\
&= \frac{1}{2} \left[ \frac{2 \sqrt{3 + t}}{\sqrt{t^2 - 1}} + \int \frac{2 \sqrt{3 + t}}{(t^2 - 1)^{\frac{3}{2}}} dt \right] \\
&= \frac{1}{2} \left[ \frac{2 \sqrt{3 + t}}{\sqrt{t^2 - 1}} + \int \frac{2 \sqrt{3 + t}}{(t - 1)(t + 1)^{\frac{3}{2}}} dt \right]
\end{align}$$

Now, let $$t - 1 = u \Rightarrow dt = du$$

Substituting this in the integral, we get

$$\begin{align}
\int \frac{dx}{x \sqrt{3 + (\ln(x))^2}} &= \frac{1}{2} \left[ \frac{2 \sqrt{3 + t}}{\sqrt{t^2 - 1}} + \int \frac{2 \sqrt{3 + t}}{(t - 1)(t + 1)^{\frac{3}{2}}} dt \right] \\
&= \frac{1}{2} \left[ \frac{2 \sqrt{3 + t}}{\sqrt{t^2 - 1}} + \int \frac{2 \sqrt{3 + t}}{u(t + 1)^{\frac{3}{2}}} du \right] \\
&= \frac{1}{2} \left[ \frac{2 \sqrt{3 + t}}{\sqrt{t^2 - 1}} + \int \frac{2 \sqrt{3 + t + 1}}{(u + 1)^{\frac{3}{2}}} du \right] \\
&= \frac{1}{2} \left[ \frac{2 \sqrt{3 + t}}{\sqrt{t^2 - 1}} + \int \frac{2 \sqrt{4 + t}}{(u + 1)^{\frac{3}{2}}} du \right]
\end{align}$$

Now, using the **Integration by Parts**, let $$u = \sqrt{4 + t} \Rightarrow dv = \frac{du}{(u + 1)^{\frac{3}{2}}}$$

and

$$\begin{align}
du &= \frac{dt}{2 \sqrt{4 + t}} \\
v &= \frac{2}{3} \frac{1}{(u + 1)^{\frac{3}{2}}}
\end{align}$$

Substituting this in the integral, we get

$$\begin{align}
\int \frac{dx}{x \sqrt{3 + (\ln(x))^2}} &= \frac{1}{2} \left[ \frac{2 \sqrt{3 + t}}{\sqrt{t^2 - 1}} + \int \frac{2 \sqrt{4 + t}}{(u + 1)^{\frac{3}{2}}} du \right] \\
&= \frac{1}{2} \left[ \frac{2 \sqrt{3 + t}}{\sqrt{t^2 - 1}} + \left[ uv - \int v du \right] \right] \\
&= \frac{1}{2} \left[ \frac{2 \sqrt{3 + t}}{\sqrt{t^2 - 1}} + \left[ \sqrt{4 + t}\frac{2}{3} \frac{1}{(u + 1)^{\frac{3}{2}}} - \int \frac{2}{3} \frac{1}{(u + 1)^{\frac{3}{2}}} du \right] \right]
\end{align}$$

Now, let $$u + 1 = v \Rightarrow du = dv$$

Substituting this in the integral, we get

$$\begin{align}
\int \frac{dx}{x \sqrt{3 + (\ln(x))^2}} &= \frac{1}{2} \left[ \frac{2 \sqrt{3 + t}}{\sqrt{t^2 - 1}} + \left[ \sqrt{4 + t}\frac{2}{3} \frac{1}{(u + 1)^{\frac{3}{2}}} - \int \frac{2}{3} \frac{1}{(u + 1)^{\frac{3}{2}}} du \right] \right] \\
&= \frac{1}{2} \left[ \frac{2 \sqrt{3 + t}}{\sqrt{t^2 - 1}} + \sqrt{4 + t}\frac{2}{3} \frac{1}{v^{\frac{3}{2}}} - \frac{2}{3}\int \frac{dv}{v^{\frac{3}{2}}} \right]
\end{align}$$

Now, using the **Integration by Parts**, let $$v^{\frac{1}{2}} = u \Rightarrow dv = 2u du$$

and

$$\begin{align}
du &= \frac{dv}{2u} \\
v &= u^2
\end{align}$$

Substituting this in the integral, we get

$$\begin{align}
\int \frac{dx}{x \sqrt{3 + (\ln(x))^2}} &= \frac{1}{2} \left[ \frac{2 \sqrt{3 + t}}{\sqrt{t^2 - 1}} + \sqrt{4 + t}\frac{2}{3} \frac{1}{v^{\frac{3}{2}}} - \frac{2}{3}\int \frac{dv}{v^{\frac{3}{2}}} \right] \\
&= \frac{1}{2} \left[ \frac{2 \sqrt{3 + t}}{\sqrt{t^2 - 1}} + \sqrt{4 + t}\frac{2}{3} \frac{1}{v^{\frac{3}{2}}} - \frac{2}{3}\left[ uv - \int v du \right] \right] \\
&= \frac{1}{2} \left[ \frac{2 \sqrt{3 + t}}{\sqrt{t^2 - 1}} + \sqrt{4 + t}\frac{2}{3} \frac{1}{v^{\frac{3}{2}}} - \frac{2}{3}\left[ u^2 \frac{dv}{2u} - \int \frac{dv}{2u} du \right] \right] \\
&= \frac{1}{2} \left[ \frac{2 \sqrt{3 + t}}{\sqrt{t^2 - 1}} + \sqrt{4 + t}\frac{2}{3} \frac{1}{v^{\frac{3}{2}}} - \frac{2}{3}\left[ u^2 \frac{dv}{2u} - \int \frac{2u du}{2u} \right] \right] \\
&= \frac{1}{2} \left[ \frac{2 \sqrt{3 + t}}{\sqrt{t^2 - 1}} + \sqrt{4 + t}\frac{2}{3} \frac{1}{v^{\frac{3}{2}}} - \frac{2}{3}\left[ u^2 \frac{dv}{2u} - u^2 \right] \right] \\
&= \frac{1}{2} \left[ \frac{2 \sqrt{3 + t}}{\sqrt{t^2 - 1}} + \sqrt{4 + t}\frac{2}{3} \frac{1}{v^{\frac{3}{2}}} - \frac{1}{3}\left[ u^2 \right] \right]
\end{align}$$

Now, substituting $t = \sec^2(\theta)$ and $u = \sqrt{4 + t}$, we get

$$\begin{align}
\int \frac{dx}{x \sqrt{3 + (\ln(x))^2}} &= \frac{1}{2} \left[ \frac{2 \sqrt{3 + \sec^2(\theta)}}{\sqrt{\sec^2(\theta) - 1}} + \sqrt{4 + \sec^2(\theta)}\frac{2}{3} \frac{1}{v^{\frac{3}{2}}} - \frac{1}{3}\left[ \sqrt{4 + \sec^2(\theta)} \right] \right] \\
&= \frac{1}{2} \left[ \frac{2 \sec(\theta)}{\sqrt{\sec^2(\theta) - 1}} + \sec(\theta)\frac{2}{3} \frac{1}{v^{\frac{3}{2}}} - \frac{1}{3}\left[ \sec(\theta) \right] \right]
\end{align}$$

Therefore, the solution to the given integral is

$$\int \frac{dx}{x \sqrt{3 + (\ln(x))^2}} = \frac{1}{2} \left[ \frac{2 \sec(\theta)}{\sqrt{\sec^2(\theta) - 1}} + \sec(\theta)\frac{2}{3} \frac{1}{v^{\frac{3}{2}}} - \frac{1}{3}\left[ \sec(\theta) \right] \right] + C$$