

**Solution:**

The derivative of the function $f(x) = \frac{x^4}{x^3-1}$ is equal to 0 when $x$ satisfies the equation

$$\frac{d}{dx}\left(\frac{x^4}{x^3-1}\right)=0$$

Using the chain rule, we can rewrite this equation as 

$$\frac{d}{dx}\left(x^4\right)\cdot \frac{1}{x^3-1}+x^4\cdot \frac{d}{dx}\left(\frac{1}{x^3-1}\right)=0$$ 

$$\Rightarrow 4x^3\cdot \frac{1}{x^3-1}-x^4\cdot \frac{3x^2}{(x^3-1)^2}=0$$

Therefore, we get the following equation

$$4x^3=x^4\cdot \frac{3x^2}{(x^3-1)^2}$$

Simplifying this equation, we get

$$\frac{4x^3}{x^4}=\frac{3x^2}{(x^3-1)^2}$$

$$\Rightarrow \frac{4}{x}=\frac{3}{(x^3-1)^2}$$

$$\Rightarrow \frac{4(x^3-1)^2}{x}=3$$

$$\Rightarrow 4x^2-4x+3=0$$

This is a quadratic equation in $x$. Solving it, we get 

$$x=\frac{4\pm \sqrt{16-12}}{2}=1 \text{ or } \frac{3}{2}$$

Therefore, the derivative of the function $f(x) = \frac{x^4}{x^3-1}$ is equal to 0 when $x = 1$ or $x = \frac{3}{2}$.