

# Solution

## Summation of n terms
Let $n$ be the number of terms in the summation. The sum of the first $n$ terms can be written as:

$$ S = \sum_{i=1}^{n} a_i = a_1 + a_2 + a_3 + \cdots + a_n $$

## Finding the value of $a_n$
The value of the $n^{th}$ term is given by 

$$a_n = \frac{S - (a_1 + a_2 + \cdots + a_{n-1})}{n}$$

Therefore,

$$a_n = \frac{S - \sum_{i=1}^{n-1} a_i}{n}$$

## Example
Let $S = 18$ and the first three terms of the summation be $5, 7, a_3$. 

Therefore,
$$a_3 = \frac{S - (5 + 7)}{3} = \frac{18 - 12}{3} = \frac{6}{3} = 2$$