

### **Solution:**

The derivative of the given function is: 

$$\frac{d}{dx}\left(\frac{x^4}{x^3-1}\right) = \frac{d}{dx}\left(x^4\right) \cdot \frac{d}{dx}\left(x^3-1\right)^{-1}$$

Using the product rule, we get: 

$$\frac{d}{dx}\left(\frac{x^4}{x^3-1}\right) = \frac{x^4 \cdot \left(-3x^2\right) + \left(4x^3\right) \cdot \left(x^3-1\right)^{-2}}{\left(x^3-1\right)^2}$$

Simplifying the above expression, we get:

$$\frac{d}{dx}\left(\frac{x^4}{x^3-1}\right) = \frac{4x^6 - 3x^4}{\left(x^3-1\right)^2}$$

For the derivative to be equal to 0, the numerator must also be 0. Therefore, we can solve for $x$ as follows:

$$4x^6 - 3x^4 = 0$$

$$4x^4\left(x^2 - \frac{3}{4}\right) = 0$$

$$x^2 - \frac{3}{4} = 0 \quad \text{or} \quad x^4 = 0$$

Therefore, the solutions of the equation are:

$$x = 0 \quad \text{or} \quad x = \pm \sqrt{\frac{3}{4}}$$