

## **Solution**

This equation is in the **general form** of a **quadratic equation**: $ax^2 + bxy + cy^2 + dx + ey + f = 0$

**Comparing** our equation to this general form, we see that:

$a = 1$

$b = 0$

$c = 25$

$d = 4$

$e = -150$

$f = 204$

We now use the following **transformation** to **simplify** the equation:

$\begin{aligned} x &= X - \frac{d}{2a} \\ y &= Y - \frac{e}{2c} \end{aligned}$

Substituting these values into our equation and simplifying, we get:

$X^2 + 25Y^2 + \frac{d^2 - 4ac}{4a} + \frac{e^2 - 4bc}{4c} = 0$

$\Rightarrow X^2 + 25Y^2 - \frac{-400}{4} + \frac{22500}{4} = 0$

$\Rightarrow X^2 + 25Y^2 + 5625 = 0$

This is now in its **canonical form**: $X^2 + 25Y^2 + C = 0$, where $C = 5625$.

## **Решение**

Это уравнение имеет форму общего **квадратичного уравнения**: $ax^2 + bxy + cy^2 + dx + ey + f = 0$

Сравнивая наше уравнение с этой общей формой, мы видим:

$a = 1$

$b = 0$

$c = 25$

$d = 4$

$e = -150$

$f = 204$

Для упрощения уравнения используем следующее **преобразование**:

$\begin{aligned} x &= X - \frac{d}{2a} \\ y &= Y - \frac{e}{2c} \end{aligned}$

Подставляя эти значения в наше уравнение и упрощая его, получаем:

$X^2 + 25Y^2 + \frac{d^2 - 4ac}{4a} + \frac{e^2 - 4bc}{4c} = 0$

$\Rightarrow X^2 + 25Y^2 - \frac{-400}{4} + \frac{22500}{4} = 0$

$\Rightarrow X^2 + 25Y^2 + 5625 = 0$

Это уравнение теперь имеет **каноническую форму**: $X^2 + 25Y^2 + C = 0$, где $C = 5625$.