

### **Solution**

Given: $$x = \ln{\left(1 - t^2\right)}$$ and $$y = \arcsin{\left(\sqrt{1 - t^2}\right)}$$

### **Calculating $\frac{d(y)}{dx}$**

By the chain rule, we can write:

$$\frac{d(y)}{dx} = \frac{d(y)}{dt}\frac{dt}{dx} $$

### **Calculating $\frac{dy}{dt}$**

Using the definition of the inverse sine function, we can write,

$$\frac{dy}{dt} = \frac{1}{\sqrt{1 - \sin^2{y}}} = \frac{1}{\sqrt{1 - (1 - t^2)}} = \frac{1}{\sqrt{t^2}} = \frac{1}{|t|} $$

### **Calculating $\frac{dt}{dx}$**

Using the definition of $x$ we can differentiate $t$ with respect to $x$ to obtain,

$$\frac{dt}{dx} = \frac{dt}{d{\left(\ln{\left(1 - t^2\right)}\right)}} = \frac{dt}{d{\left(1 - t^2\right)}}\frac{d{\left(1 - t^2\right)}}{d{\left(\ln{\left(1 - t^2\right)}\right)}} = \frac{-2t}{1 - t^2} \cdot \frac{1}{\ln{\left(1 - t^2\right)}} = -\frac{2t}{\ln{\left(1 - t^2\right)}} $$

### **Combining Results**

Substituting the results of the above three calculations into the expression for $\frac{d(y)}{dx}$, we get

$$\frac{d(y)}{dx} = -\frac{t}{|t|\ln{\left(1 - t^2\right)}}$$

### **Calculating $\frac{(d(y))^2}{(dx)^2}$**

Using the above result and the chain rule, we can calculate $\frac{(d(y))^2}{(dx)^2}$ as follows

$$\frac{(d(y))^2}{(dx)^2} = \frac{d{\left(\frac{t}{|t|\ln{\left(1 - t^2\right)}}\right)}}{dx} = \frac{d{\left(\frac{t}{|t|\ln{\left(1 - t^2\right)}}\right)}}{dt}\frac{dt}{dx}$$

### **Calculating $\frac{d{\left(\frac{t}{|t|\ln{\left(1 - t^2\right)}}\right)}}{dt}$**

Again, using the chain rule, we can write

$$\frac{d{\left(\frac{t}{|t|\ln{\left(1 - t^2\right)}}\right)}}{dt} = \frac{d{\left(\frac{t}{|t|}\right)}}{dt}\frac{d{\ln{\left(1 - t^2\right)}}}{dt}$$

*Note: Since $|t|$ is a constant, $\frac{d{\left(\frac{t}{|t|}\right)}}{dt} = 0$*

### **Calculating $\frac{d{\ln{\left(1 - t^2\right)}}}{dt}$**

Using the chain rule and the definition of $x$, we can write

$$\frac{d{\ln{\left(1 - t^2\right)}}}{dt} = \frac{d{\ln{\left(1 - t^2\right)}}}{d{\left(1 - t^2\right)}}\frac{d{\left(1 - t^2\right)}}{dt} = \frac{1}{1 - t^2}\cdot(-2t) = -\frac{2t}{1 - t^2}$$

### **Combining Results**

Substituting the results of the above two calculations into the expression for $\frac{d{\left(\frac{t}{|t|\ln{\left(1 - t^2\right)}}\right)}}{dt}$, we get

$$\frac{d{\left(\frac{t}{|t|\ln{\left(1 - t^2\right)}}\right)}}{dt} = 0 \cdot -\frac{2t}{1 - t^2} = 0$$

### **Final Result**

Substituting the result for $\frac{d{\left(\frac{t}{|t|\ln{\left(1 - t^2\right)}}\right)}}{dt}$ and the result for $\frac{dt}{dx}$ into the expression for $\frac{(d(y))^2}{(dx)^2}$, we get

$$\frac{(d(y))^2}{(dx)^2} = 0 \cdot -\frac{2t}{\ln{\left(1 - t^2\right)}} = 0$$

### **Russian Explanation**

Дано: $$x = \ln{\left(1 - t^2\right)}$$ и $$y = \arcsin{\left(\sqrt{1 - t^2}\right)}$$

### **Вычисление $\frac{d(y)}{dx}$**

Применив правило цепочки, мы можем написать:

$$\frac{d(y)}{dx} = \frac{d(y)}{dt}\frac{dt}{dx} $$

### **Вычисление $\frac{dy}{dt}$**

Используя определение обратного синуса, мы можем написать,

$$\frac{dy}{dt} = \frac{1}{\sqrt{1 - \sin^2{y}}} = \frac{1}{\sqrt{1 - (1 - t^2)}} = \frac{1}{\sqrt{t^2}} = \frac{1}{|t|} $$

### **Вычисление $\frac{dt}{dx}$**

Используя определение $x$ мы можем дифференцировать $t$ по отношению к $x$, чтобы получить

$$\frac{dt}{dx} = \frac{dt}{d{\left(\ln{\left(1 - t^2\right)}\right)}} = \frac{dt}{d{\left(1 - t^2\right)}}\frac{d{\left(1 - t^2\right)}}{d{\left(\ln{\left(1 - t^2\right)}\right)}} = \frac{-2t}{1 - t^2} \cdot \frac{1}{\ln{\left(1 - t^2\right)}} = -\frac{2t}{\ln{\left(1 - t^2\right)}} $$

### **Объединение результатов**

Подставляя результаты вышеописанных трех вычислений в выражение для $\frac{d(y)}{dx}$, мы получим

$$\frac{d(y)}{dx} = -\frac{t}{|t|\ln{\left(1 - t^2\right)}}$$

### **Вычисление $\frac{(d(y))^2}{(dx)^2}$**

Используя вышеуказанный результат и правило цепочки, мы можем вычислить $\frac{(d(y))^2}{(dx)^2}$ следующим образом

$$\frac{(d(y))^2}{(dx)^2} = \frac{d{\left(\frac{t}{|t|\ln{\left(1 - t^2\right)}}\right)}}{dx} = \frac{d{\left(\frac{t}{|t|\ln{\left(1 - t^2\right)}}\right)}}{dt}\frac{dt}{dx}$$

### **Вычисление $\frac{d{\left(\frac{t}{|t|\ln{\left(1 - t^2\right)}}\right)}}{dt}$**

Опять же, используя правило цепочки, мы можем написать

$$\frac{d{\left(\frac{t}{|t|\ln{\left(1 - t^2\right)}}\right)}}{dt} = \frac{d{\left(\frac{t}{|t|}\right)}}{dt}\frac{d{\ln{\left(1 - t^2\right)}}}{dt}$$

*Примечание: Так как $|t|$ является константой, $\frac{d{\left(\frac{t}{|t|}\right)}}{dt} = 0$*

### **Вычисление $\frac{d{\ln{\left(1 - t^2\right)}}}{dt}$**

Используя правило цепочки и определение $x$, мы можем написать

$$\frac{d{\ln{\left(1 - t^2\right)}}}{dt} = \frac{d{\ln{\left(1 - t^2\right)}}}{d{\left(1 - t^2\right)}}\frac{d{\left(1 - t^2\right)}}{dt} = \frac{1}{1 - t^2}\cdot(-2t) = -\frac{2t}{1 - t^2}$$

### **Объединение результатов**

Подставляя результаты вышеуказанных двух вычислений в выражение для $\frac{d{\left(\frac{t}{|t|\ln{\left(1 - t^2\right)}}\right)}}{dt}$, мы получим

$$\frac{d{\left(\frac{t}{|t|\ln{\left(1 - t^2\right)}}\right)}}{dt} = 0 \cdot -\frac{2t}{1 - t^2} = 0$$

### **Финальный результат**

Подставляя результат для $\frac{d{\left(\frac{t}{|t|\ln{\left(1 - t^2\right)}}\right)}}{dt}$ и результат для $\frac{dt}{dx}$ в выражение для $\frac{(d(y))^2}{(dx)^2}$, мы получим

$$\frac{(d(y))^2}{(dx)^2} = 0 \cdot -\frac{2t}{\ln{\left(1 - t^2\right)}} = 0$$