

**Solution**

We can use integration by parts to solve this integral.

$$\int \tan^4(x) \frac{1}{\cos^4(x)} dx$$

Let $u = \tan^4(x)$ and $dv = \frac{1}{\cos^4(x)}dx$.

Then, $du = 4\tan^3(x)\sec^2(x)dx$ and $v = -\frac{1}{3}\tan^3(x)$.

We can now apply integration by parts:

$$\int udv = uv - \int vdu$$

$$\int \tan^4(x) \frac{1}{\cos^4(x)} dx = -\frac{1}{3}\tan^3(x)\tan^4(x) + \int -\frac{4}{3}\tan^3(x)\tan^3(x)\sec^2(x)dx$$

Now, let $u = \tan^3(x)$ and $dv = \tan(x)\sec^2(x)dx$.

Then, $du = 3\tan^2(x)\sec^2(x)dx$ and $v = -\frac{1}{2}\sec^2(x)$.

We can apply integration by parts again:

$$\int -\frac{4}{3}\tan^3(x)\tan^3(x)\sec^2(x)dx = -\frac{2}{3}\tan^3(x)\sec^2(x) + \int -\frac{6}{2}\tan^2(x)\sec^2(x)\sec^2(x)dx$$

Finally, let $u = \tan^2(x)$ and $dv = \sec^4(x)dx$.

Then, $du = 2\tan(x)\sec^2(x)dx$ and $v = -\frac{1}{5}\sec^4(x)$.

We can apply integration by parts for the last time:

$$\int -\frac{6}{2}\tan^2(x)\sec^2(x)\sec^2(x)dx = -\frac{3}{5}\tan^2(x)\sec^4(x) + \int -\frac{6}{5}\tan(x)\sec^4(x)dx$$

Now, we can combine all of the integrals:

$$\int \tan^4(x) \frac{1}{\cos^4(x)} dx = -\frac{1}{3}\tan^3(x)\tan^4(x) - \frac{2}{3}\tan^3(x)\sec^2(x) - \frac{3}{5}\tan^2(x)\sec^4(x) + \int -\frac{6}{5}\tan(x)\sec^4(x)dx$$

Therefore, the solution to the integral is:

$$-\frac{1}{3}\tan^3(x)\tan^4(x) - \frac{2}{3}\tan^3(x)\sec^2(x) - \frac{3}{5}\tan^2(x)\sec^4(x) + \int -\frac{6}{5}\tan(x)\sec^4(x)dx$$