

## **Solution**

The given differential equation is:

$$y'' + y = 6 \sin (2x)$$

This equation is linear and homogeneous, so we can look for solutions of the form $y = \text{A}\sin\left(2x\right) + \text{B}\cos\left(2x\right)$.

## **Step 1: Differentiate the proposed solution**

Differentiating the proposed solution, we get

$$y' = 2\text{A}\cos(2x) - 2\text{B}\sin(2x)$$

$$y'' = -4\text{A}\sin(2x) - 4\text{B}\cos(2x)$$

Substituting these derivatives into the original equation gives 

$$-4\text{A}\sin(2x) - 4\text{B}\cos(2x) + \text{A}\sin\left(2x\right) + \text{B}\cos\left(2x\right) = 6 \sin (2x)$$

## **Step 2: Simplify the equation**

Simplifying the above equation, we get

$$-3\text{A}\sin(2x) - 3\text{B}\cos(2x) = 6 \sin (2x)$$

## **Step 3: Solve for the coefficients**

For the equation to be true for all values of $x$, the coefficients $\text{A}$ and $\text{B}$ must be chosen such that the coefficients of $\sin(2x)$ and $\cos(2x)$ are equal.

Therefore, 

$$-3\text{A} = 6 \implies \text{A} = -2$$

$$-3\text{B} = 0 \implies \text{B} = 0$$

## **Step 4: Write down the solution**

The solution of the differential equation is given by

$$y = -2\sin\left(2x\right)$$