

# **Solution**

We can write the given expression in trigonometric form using Euler's formula:

$e^{ix} = \cos x + i\sin x$

$e^{-ix} = \cos (-x) + i\sin (-x)$

Substituting this in the given expression, we get

$e^{ix} + e^{-ix} = \cos x + i\sin x + \cos (-x) + i\sin (-x)$

Using the trigonometric identity $\cos (-x) = \cos x$ and $\sin (-x) = -\sin x$, we get

$e^{ix} + e^{-ix} = 2\cos x + i\sin x - i\sin x$

Simplifying the above expression, we get

$e^{ix} + e^{-ix} = 2\cos x$

Thus, the given expression can be written in trigonometric form as

$e^{ix} + e^{-ix} = 2\cos x$