

**Solution:**

Let's use the method of undetermined coefficients to solve the given differential equation.

The general solution of the differential equation is given by:

$$y=C_1\cos x + C_2\sin x$$

where $C_1$ and $C_2$ are arbitrary constants.

**Step 1:**

Let's assume a particular solution of the form:

$$y=A\cos x + B\sin x$$

**Step 2:**

Substituting this particular solution into the given differential equation, we get:

$$A\cos x + B\sin x + \cos x + \sin x = 0$$

$$\implies A\cos x + B\sin x = -(\cos x + \sin x)$$

**Step 3:**

Comparing the coefficients of $\cos x$ and $\sin x$, we get:

$$A = -1 \hspace{2cm} \text{and} \hspace{2cm} B = -1$$

**Step 4:**

Therefore, the particular solution of the given differential equation is:

$$y=-\cos x - \sin x$$

**Step 5:**

The general solution of the differential equation is given by:

$$y=C_1\cos x + C_2\sin x - \cos x - \sin x$$

**Step 6:**

Rearranging the terms, we get:

$$y=(C_1 - 1)\cos x + (C_2 - 1)\sin x$$

Therefore, the general solution of the given differential equation is:

$$y=C_1\cos x + C_2\sin x$$