

### Solution

The given expression can be reduced to a linear form as follows:

$$Y = \frac{e^{B_1 + B_2X_i + E_i}}{1 + e^{B_1 + B_2X_i + E_i}}$$

Let $$Z = e^{B_1 + B_2X_i + E_i}$$

Then $$Y = \frac{Z}{1+Z}$$

Or $$Y(1+Z) = Z$$

Or $$Y + YZ = Z$$

Or $$Y(1+Z) - YZ = Z - YZ$$

Or $$Y = \frac{Z - YZ}{1+Z}$$

Or $$Y = \frac{e^{B_1 + B_2X_i + E_i} - Ye^{B_1 + B_2X_i + E_i}}{1 + e^{B_1 + B_2X_i + E_i}}$$

Or $$Y(1 + e^{B_1 + B_2X_i + E_i}) = e^{B_1 + B_2X_i + E_i}$$

Or $$Y = \frac{e^{B_1 + B_2X_i + E_i}}{1 + e^{B_1 + B_2X_i + E_i}}$$