

**Solution:**

The derivative of the function $f(x) = \frac{x^4}{x^3 - 1}$ is given by 

$$f'(x) = \frac{4x^3(x^3 - 1) - x^4(3x^2)}{(x^3 - 1)^2} = \frac{x^4(x^3 - 4)}{(x^3 - 1)^2}$$

To find where $f'(x) = 0$, we set the numerator equal to 0 and solve for $x$:

$$x^4(x^3 - 4) = 0$$

$$x^3(x^3 - 4) = 0$$

$$x^3 = 0 \text{ or } x^3 - 4 = 0$$

$$x = 0 \text{ or } x^3 = 4$$

$$x = 0 \text{ or } x = \sqrt[3]{4}$$

Therefore, the derivative of the function $f(x) = \frac{x^4}{x^3 - 1}$ is equal to 0 when $x = 0$ and $x = \sqrt[3]{4}$.