

**Solution:** 

We need to use integration by parts. 

Let $u = \tan^{4}(x)$ and $dv = \frac{1}{\cos^{4}(x)}dx$. 

Then $du = 4\tan^{3}(x)\sec^{2}(x)dx$ and $v = \frac{1}{3\cos^{3}(x)}$. 

Therefore, 
\begin{align}
\int \tan^{4}(x)\frac{1}{\cos^{4}(x)}dx &= \frac{1}{3}\tan^{4}(x)\frac{1}{\cos^{3}(x)} - \frac{4}{3}\int \tan^{3}(x)\sec^{2}(x)\frac{1}{\cos^{3}(x)}dx \\
&= \frac{1}{3}\tan^{4}(x)\frac{1}{\cos^{3}(x)} - \frac{4}{3}\int \sec^{2}(x)\tan^{2}(x)dx \\
&= \frac{1}{3}\tan^{4}(x)\frac{1}{\cos^{3}(x)} - \frac{2}{3}\int \tan^{2}(x)\sec^{2}(x)dx \\
&= \frac{1}{3}\tan^{4}(x)\frac{1}{\cos^{3}(x)} - \frac{2}{3}\int \frac{\tan^{2}(x)}{\cos^{2}(x)}dx \\
&= \frac{1}{3}\tan^{4}(x)\frac{1}{\cos^{3}(x)} - \frac{2}{3}\int \frac{\sec^{2}(x)-1}{\cos^{2}(x)}dx \\
&= \frac{1}{3}\tan^{4}(x)\frac{1}{\cos^{3}(x)} - \frac{2}{3}\int \sec^{2}(x)dx + \frac{2}{3}\int \frac{1}{\cos^{2}(x)}dx \\
&= \frac{1}{3}\tan^{4}(x)\frac{1}{\cos^{3}(x)} - \frac{2}{3}\tan(x) + \frac{2}{3}\sec(x) + C
\end{align}