

# Производная от $$2 \frac{x^{-1}}{2x}$$

Используем правило цепной дифференциации:

$$\frac{d}{dx}\left(2 \frac{x^{-1}}{2x}\right)=\frac{d}{dx}\left(2\right)\frac{x^{-1}}{2x}+2\frac{d}{dx}\left(x^{-1}\right)\frac{1}{2x}+2\frac{x^{-1}}{2x}\frac{d}{dx}\left(2x\right)$$

Далее подставляем значения производных:

$$\frac{d}{dx}\left(2 \frac{x^{-1}}{2x}\right)=0 \cdot \frac{x^{-1}}{2x}+2\cdot(-1)x^{-2}\cdot\frac{1}{2x}+2\cdot \frac{x^{-1}}{2x}\cdot 2= -2x^{-2}$$

Ответ:

$$\frac{d}{dx}\left(2 \frac{x^{-1}}{2x}\right)=-2x^{-2}$$