

**Solution**

Using Ito's formula, the process $X_t$ can be written as:

$$dX_t = \frac{\partial X_t}{\partial t} dt + \frac{\partial X_t}{\partial W_t} dW_t + \frac{1}{2}\frac{\partial^2 X_t}{\partial W_t^2} dW_t^2$$

Substituting in the given process $X_t$, we get:

$$dX_t = t^2 \frac{\partial W_t^3}{\partial t} dt + t^2 \frac{\partial W_t^3}{\partial W_t} dW_t + \frac{1}{2}t^2 \frac{\partial^2 W_t^3}{\partial W_t^2} dW_t^2$$

Using the following identities,

$$\frac{\partial W_t^3}{\partial t}=0, \quad \frac{\partial W_t^3}{\partial W_t}=3W_t^2, \quad \frac{\partial^2 W_t^3}{\partial W_t^2}=6W_t$$

we get

$$dX_t = 3t^2 W_t^2 dW_t + 3t^2 W_t dW_t^2$$

$$dX_t = (3t^2 W_t^2 - 3t^2 W_t)dW_t + 3t^2 W_t dW_t^2$$

$$dX_t = G_t dt + H_t dW_t$$

where,

$$G_t = 0, \quad H_t = 3t^2 W_t^2 - 3t^2 W_t$$

Therefore, the process $X_t$ can be represented in the form $dX_t = G_t dt + H_t dW_t$.