

**Solution of the Integral without Using Substitution Method**

We start by factoring the denominator of the expression:

$$\int \frac{dx}{x \sqrt{3 + (\ln x)^2}} = \int \frac{dx}{x \sqrt{3} \sqrt{1 + \left(\frac{\ln x}{\sqrt{3}}\right)^2}}$$

Now, using the trigonometric substitution $u = \frac{\ln x}{\sqrt{3}}$, we get $du = \frac{1}{\sqrt{3} \, x} \, dx$. Then, the integral becomes:

$$\int \frac{dx}{x \sqrt{3} \sqrt{1 + \left(\frac{\ln x}{\sqrt{3}}\right)^2}} = \int \frac{du}{\sqrt{1 + u^2}}$$

Using the integral identity $\int \frac{du}{\sqrt{1 + u^2}} = \sin^{-1} u + C$, we get:

$$\int \frac{dx}{x \sqrt{3} \sqrt{1 + \left(\frac{\ln x}{\sqrt{3}}\right)^2}} = \sin^{-1}\left(\frac{\ln x}{\sqrt{3}}\right) + C$$

Therefore, the solution to the given integral is 

$$\boxed{\int \frac{dx}{x \sqrt{3 + (\ln x)^2}} = \sin^{-1}\left(\frac{\ln x}{\sqrt{3}}\right) + C}$$